proof/AdequacyLocal.v
@@ -1,8 +1,5 @@
 Require Import CoqlibC.
 Require Import Simulation.
-Require Import Skeleton.
-Require Import Sem.
-Require Import ModSem.
 Require Import LinkingC.
 Require Import Skeleton.
 Require Import Values.
@@ -11,19 +8,43 @@ Require Import Asmregs.
 Require Import Smallstep.
 Require Import Integers.
 
+Require Import Skeleton ModSem Mod Sem.
 Require Import SimDef SimSymb SimMem SimMod SimModSem SimProg SimLoad SimProg.
 Require Import Ord.
 
 Set Implicit Arguments.
 
 
+Definition bar_True: Type := True.
+Global Opaque bar_True.
 Ltac bar :=
   let NAME := fresh
                 "TTTTTTTTTTTTTTTTTTTTTTTTTTTTTTTTTTTTTTTTTTTTTTTTTTTTTTTTTTTTTTTTTTTTTTTTTTTTTTTTTTTTTTTTTTTTTTTTTTTTTT"
   in
-  assert(NAME: True) by ss
+  assert(NAME: bar_True) by ss
 .
 (* TODO: Move to CoqlibC *)
+
+Ltac clear_until id :=
+  on_last_hyp ltac:(fun id' => match id' with
+                               | id => idtac
+                               | _ => clear id'; clear_until id
+                               end)
+.
+
+Ltac clear_until_bar :=
+  on_last_hyp ltac:(fun id' => match (type of id') with
+                               | bar_True => idtac
+                               | _ => clear id'; clear_until_bar
+                               end)
+.
+
+Goal True -> True -> False.
+  intro. bar. intro.
+  clear_until H0. clear_until H. Undo 2.
+  clear_until_bar.
+  clear_tac.
+Abort.
 
 
 
@@ -46,6 +67,196 @@ Section INITDTM.
   Variable p: program.
   Let sem := Sem.semantics p.
 
+  Lemma skenv_link_wf
+        sk_link
+        (LINKSK: link_sk p = Some sk_link)
+    :
+      <<WF: SkEnv.wf sk_link.(Sk.load_skenv)>>
+  .
+  Proof.
+    u.
+    admit "easy. follow induction proofs on Globalenvs.v".
+  Qed.
+
+  Lemma system_disjoint
+        skenv_link
+        (WFBIG: SkEnv.wf skenv_link)
+        sys_def
+        fptr
+        (SYSTEM: Genv.find_funct (System.skenv skenv_link) fptr = Some (Internal sys_def))
+        md md_def
+        (MOD: In md p)
+        (MODSEM: Genv.find_funct (ModSem.skenv (Mod.get_modsem md skenv_link (Mod.data md))) fptr =
+                 Some (Internal md_def))
+    :
+      False
+  .
+  Proof.
+    erewrite <- Mod.get_modsem_projected_sk in *.
+    hexploit (SkEnv.project_impl_spec skenv_link (defs (Mod.get_sk md (Mod.data md)))); eauto. intro SPEC.
+    remember (SkEnv.project skenv_link (defs (Mod.get_sk md (Mod.data md)))) as skenv_proj eqn:T in *.
+    assert(WFSMALL: skenv_proj.(SkEnv.wf)).
+    { eapply SkEnv.project_spec_preserves_wf; eauto. }
+    clarify. des. inv SPEC.
+    exploit Genv.find_funct_inv; eauto. i; des. clarify. ss. des_ifs.
+    unfold Genv.find_funct_ptr in *. des_ifs.
+    inv WFSMALL. exploit DEFSYMB; eauto. intro SYMBSMALL; des.
+    assert((defs (Mod.get_sk md (Mod.data md))) id).
+    { apply NNPP. ii.
+      exploit SYMBDROP; eauto. i; des. clarify.
+    }
+    exploit SYMBKEEP; eauto. intro SYMBBIG; des.
+    rewrite SYMBSMALL in *. symmetry in SYMBBIG.
+    exploit DEFKEEP; eauto.
+    { eapply Genv.find_invert_symbol; eauto. }
+    intro DEFSMALL; des. rewrite Heq in *. symmetry in DEFSMALL.
+    clear - Heq0 DEFSMALL.
+    unfold System.skenv in *. ss.
+    exploit Genv_map_defs_spec; eauto. i; des. unfold System.gd_to_skd in MAP. des_ifs.
+    clear Heq0.
+    exploit Genv_map_defs_spec; eauto. i; des. des_ifs.
+  Qed.
+
+  (* Lemma link_sk_disjoint_aux *)
+  (*       (sks: list Sk.t) *)
+  (*       sk0 sk1 *)
+  (*       (IN0: In sk0 sks) *)
+  (*       (IN1: In sk1 sks) *)
+  (*       sk_link *)
+  (*       (LINKSK: link_list sks = Some sk_link) *)
+  (*       (NEQ: sk0 <> sk1) *)
+  (*   : *)
+  (*     sk0.(defs) /1\ sk1.(defs) <1= bot1 *)
+  (* . *)
+  (* Proof. *)
+  (*   admit "". *)
+  (* Qed. *)
+
+  (* Lemma link_sk_disjoint *)
+  (*       md0 md1 *)
+  (*       (IN0: In md0 p) *)
+  (*       (IN1: In md1 p) *)
+  (*       sk_link *)
+  (*       (LINKSK: link_sk p = Some sk_link) *)
+  (*       (NEQ: md0.(Mod.sk) <> md1.(Mod.sk)) *)
+  (*   : *)
+  (*     md0.(Mod.sk).(defs) /1\ md1.(Mod.sk).(defs) <1= bot1 *)
+  (* . *)
+  (* Proof. *)
+  (*   unfold link_sk in *. *)
+  (*   hexploit link_sk_disjoint_aux; eauto. *)
+  (*   { rewrite in_map_iff. esplits; eauto. } *)
+  (*   { rewrite in_map_iff. esplits; eauto. } *)
+  (* Qed. *)
+
+  Lemma link_sk_disjoint
+        md0 md1
+        (IN0: In md0 p)
+        (IN1: In md1 p)
+        sk_link
+        (LINKSK: link_sk p = Some sk_link)
+        (NEQ: md0 <> md1)
+    :
+      md0.(Mod.sk).(defs) /1\ md1.(Mod.sk).(defs) <1= bot1
+  .
+  Proof.
+    clear_tac. clear sem.
+    unfold link_sk in *.
+    unfold Mod.sk in *.
+    ginduction p; i; ss.
+    eapply link_list_cons_inv in LINKSK. des_safe.
+    hexploit (link_list_linkorder _ TL); eauto. intro TLORD; des_safe.
+    hexploit (link_linkorder _ _ _ HD); eauto. intro HDORD; des_safe.
+
+    destruct IN0; ss.
+    { clarify. des; ss.
+Local Transparent Linker_prog.
+      simpl in HD. simpl in TL.
+      ss.
+(* Local Opaque Linker_prog. *)
+(*       exploit link_prog_inv; eauto. *)
+(*       unfold Linker_prog in *. *)
+(*     } *)
+  Abort.
+
+  Theorem genv_disjoint
+    :
+      <<DISJ: sem.(globalenv).(Ge.disjoint)>>
+  .
+  Proof.
+    ss. des_ifs; cycle 1.
+    { econs; eauto. ii; ss. inv FIND0. ss. }
+    assert(WFBIG: t.(Sk.load_skenv).(SkEnv.wf)).
+    { eapply skenv_link_wf; eauto. }
+    econs; eauto.
+    ii; ss.
+    inv FIND0; inv FIND1.
+    unfold Sk.load_skenv in *. unfold load_genv in *. unfold load_modsems in *. ss.
+    abstr (Genv.globalenv t) skenv_link. rename t into sk_link.  rename Heq into SKLINK.
+    rewrite in_map_iff in *.
+    u in *.
+    destruct MODSEM.
+    { clarify. des; ss. exfalso. clarify. eapply system_disjoint; eauto. }
+    des; ss.
+    { clarify. ss. exfalso. eapply system_disjoint; eauto. }
+
+    rename x into md0. rename x0 into md1.
+    clarify.
+    destruct fptr; ss. des_ifs. unfold Genv.find_funct_ptr in *. des_ifs.
+    rename Heq0 into DEF0. rename Heq into DEF1.
+    rewrite <- Mod.get_modsem_projected_sk in *.
+    hexploit (SkEnv.project_impl_spec skenv_link (defs (Mod.get_sk md0 (Mod.data md0)))); eauto. intro SPEC0.
+    hexploit (SkEnv.project_impl_spec skenv_link (defs (Mod.get_sk md1 (Mod.data md1)))); eauto. intro SPEC1.
+    des.
+
+    assert(WFSMALL0: (SkEnv.project skenv_link (defs (Mod.get_sk md0 (Mod.data md0)))).(SkEnv.wf)).
+    { eapply SkEnv.project_spec_preserves_wf; try apply SPEC0; eauto. }
+    assert(WFSMALL1: (SkEnv.project skenv_link (defs (Mod.get_sk md1 (Mod.data md1)))).(SkEnv.wf)).
+    { eapply SkEnv.project_spec_preserves_wf; try apply SPEC1; eauto. }
+
+    bar.
+    inv WFSMALL0. exploit DEFSYMB; eauto. i; des.
+    inv WFSMALL1. exploit DEFSYMB0; eauto. i; des.
+    rename H into SYMB0. rename H1 into SYMB1. rename id0 into id1. rename id into id0.
+    move SYMB0 at top. move SYMB1 at top. clear_until_bar.
+
+    inv SPEC0.
+    assert(DEFS0: defs (Mod.get_sk md0 (Mod.data md0)) id0).
+    { apply NNPP. ii. exploit SYMBDROP; eauto. i; des. clarify. }
+    exploit SYMBKEEP; eauto. intro SYMBBIG0; des. rewrite SYMB0 in *. symmetry in SYMBBIG0.
+    exploit DEFKEEP; eauto.
+    { eapply Genv.find_invert_symbol; eauto. }
+    intro DEFBIG0; des. rewrite DEF0 in *. symmetry in DEFBIG0.
+    move SYMBBIG0 at top.
+    move DEFBIG0 at top.
+    move DEFS0 at top.
+    clear_until_bar.
+
+    inv SPEC1.
+    assert(DEFS1: defs (Mod.get_sk md1 (Mod.data md1)) id1).
+    { apply NNPP. ii. exploit SYMBDROP; eauto. i; des. clarify. }
+    exploit SYMBKEEP; eauto. intro SYMBBIG1; des. rewrite SYMB1 in *. symmetry in SYMBBIG1.
+    exploit DEFKEEP; eauto.
+    { eapply Genv.find_invert_symbol; eauto. }
+    intro DEFBIG1; des. rewrite DEF1 in *. symmetry in DEFBIG1.
+    move SYMBBIG1 at top.
+    move DEFBIG1 at top.
+    move DEFS1 at top.
+    clear_until_bar.
+
+    assert(id0 = id1).
+    { eapply Genv.genv_vars_inj.
+      { apply SYMBBIG0. }
+      { apply SYMBBIG1. }
+    } clarify.
+    rename id1 into id.
+
+    clear - DEF0 DEF1 DEFBIG0 DEFS0 DEFS1 SKLINK H0 MODSEM1.
+    destruct (classic (md0 = md1)); ss.
+    { clarify. }
+    admit "this should hold. state some lemma like: link_sk_disjoint".
+  Qed.
+
   Lemma find_fptr_owner_determ
         fptr ms0 ms1
         (FIND0: Ge.find_fptr_owner sem.(globalenv) fptr ms0)
@@ -59,14 +270,15 @@ Section INITDTM.
     admit "use Mod.get_modsem_projected_sk".
   Qed.
 
-  Theorem initial_determ
+  Theorem initial_state_determ
           st_init0 st_init1
-          (INIT0: sem.(initial_state) st_init0)
-          (INIT1: sem.(initial_state) st_init1)
+          (INIT0: sem.(Smallstep.initial_state) st_init0)
+          (INIT1: sem.(Smallstep.initial_state) st_init1)
     :
       st_init0 = st_init1
   .
   Proof.
+    ss.
     inv INIT0; inv INIT1; ss.
     clarify.
     exploit find_fptr_owner_determ; ss; des_ifs.
@@ -97,12 +309,31 @@ Section SIMGE.
   Context {SS: SimSymb.class SM}.
   (* Inductive sim_gepair (sm0: SimMem.t) (ge_src ge_tgt: list ModSem.t): Prop := *)
   Inductive sim_ge (sm0: SimMem.t): Ge.t -> Ge.t -> Prop :=
-  | intro_sim_gepair
+  | sim_ge_src_stuck
+      ge_tgt
+    :
+      sim_ge sm0 [] ge_tgt
+  | sim_ge_intro
       msps
       (SIMSKENV: List.Forall (fun msp => ModSemPair.sim_skenv msp sm0) msps)
       (SIMMSS: List.Forall (ModSemPair.sim) msps)
+      ge_src ge_tgt
+      (GESRC: ge_src = (map (ModSemPair.src) msps))
+      (GETGT: ge_tgt = (map (ModSemPair.tgt) msps))
     :
-      sim_ge sm0 (map (ModSemPair.src) msps) (map (ModSemPair.tgt) msps)
+      sim_ge sm0 ge_src ge_tgt 
+  (* | sim_ge_intro *)
+  (*     msps *)
+  (*     (SIMSKENV: List.Forall (fun msp => ModSemPair.sim_skenv msp sm0) msps) *)
+  (*     (SIMMSS: List.Forall (ModSemPair.sim) msps) *)
+  (*     ge_src ge_tgt *)
+  (*     skenv_link_src skenv_link_tgt *)
+  (*     (GESRC: ge_src = System.modsem skenv_link_src :: (map (ModSemPair.src) msps)) *)
+  (*     (GETGT: ge_tgt = System.modsem skenv_link_tgt :: (map (ModSemPair.tgt) msps)) *)
+  (*     ss_link *)
+  (*     (SIMSYS: SimSymb.sim_skenv sm0 ss_link skenv_link_src skenv_link_tgt) *)
+  (*   : *)
+  (*     sim_ge sm0 ge_src ge_tgt  *)
   .
 
 
@@ -116,12 +347,14 @@ Section SIMGE.
         (FINDSRC: Ge.find_fptr_owner ge_src fptr_src ms_src)
     :
       exists msp,
-        <<FINDTGT: Ge.find_fptr_owner ge_tgt fptr_tgt msp.(ModSemPair.tgt)>>
+        <<SRC: msp.(ModSemPair.src) = ms_src>>
+        /\ <<FINDTGT: Ge.find_fptr_owner ge_tgt fptr_tgt msp.(ModSemPair.tgt)>>
         /\ <<SIMMS: ModSemPair.sim msp>>
         /\ <<SIMSKENV: ModSemPair.sim_skenv msp sm0>>
   .
   Proof.
     inv SIMGE.
+    { inv FINDSRC; ss. }
     rewrite Forall_forall in *.
     inv FINDSRC.
     rewrite in_map_iff in MODSEM. des. rename x into msp.
@@ -130,11 +363,8 @@ Section SIMGE.
     specialize (SIMMSS msp). exploit SIMMSS; eauto. clear SIMMSS. intro SIMMS.
     specialize (SIMSKENV msp). exploit SIMSKENV; eauto. clear SIMSKENV. intro SIMSKENV.
 
-    exploit SimSymb.sim_skenv_def_fsim; eauto. intro SIMDEF; des.
-    inv SIMDEF. exploit DEFFSIM; eauto. i; des. clear_tac. inv SIM. inv SIM0.
-   
-    assert(exists blk_tgt, fptr_tgt = Vptr blk_tgt Ptrofs.zero true).
-    { inv SAFESRC. esplits; eauto. } clear SAFESRC. des. clarify.
+    exploit SimSymb.sim_skenv_func_fsim; eauto. intro SIMFUNC; des.
+    inv SIMFUNC. exploit FUNCSIM; eauto. i; des. clear_tac. inv SIM.
     econs; eauto.
     - apply in_map_iff. esplits; eauto.
  
@@ -142,7 +372,7 @@ Section SIMGE.
  
 
 
-  Lemma find_fptr_owner_bsim
+  Lemma find_fptr_owner_bsim_deprecated
         sm0 ge_src ge_tgt
         (SIMGE: sim_ge sm0 ge_src ge_tgt)
         fptr_src fptr_tgt
@@ -159,24 +389,29 @@ Section SIMGE.
   .
   Proof.
     inv SIMGE.
+    { des. inv SAFESRC; ss. }
     rewrite Forall_forall in *.
-    inv FINDTGT.
-    rewrite in_map_iff in MODSEM. des. rename x into msp.
-    esplits; eauto.
-    clarify.
-    specialize (SIMMSS msp). exploit SIMMSS; eauto. clear SIMMSS. intro SIMMS.
-    specialize (SIMSKENV msp). exploit SIMSKENV; eauto. clear SIMSKENV. intro SIMSKENV.
-    assert(exists blk_src, fptr_src = Vptr blk_src Ptrofs.zero true).
-    { inv SAFESRC. esplits; eauto. } clear SAFESRC. des. clarify.
-    exploit SimSymb.sim_skenv_def_bsim; eauto. intro SIMDEF; des.
-    inv SIMDEF. exploit DEFBSIM; eauto. i; des. clear_tac. inv SIM. inv SIM0.
-    econs; eauto.
-    - apply in_map_iff. esplits; eauto.
+    {
+      des.
+      inv SAFESRC.
+      rewrite in_map_iff in MODSEM. des. rename x into msp.
+      clarify.
+
+      specialize (SIMMSS msp). exploit SIMMSS; eauto. clear SIMMSS. intro SIMMS.
+      specialize (SIMSKENV msp). exploit SIMSKENV; eauto. clear SIMSKENV. intro SIMSKENV.
+      exploit SimSymb.sim_skenv_func_bsim; eauto. intro SIMFUNC; des.
+      inv SIMFUNC.
+      exploit FUNCPROGRESS; eauto. i; des.
+      exploit FUNCBSIM; try apply PROGRESS; eauto. i; des. clarify. clear_tac. inv SIM.
+      exists msp. esplits; eauto.
+      { econs; eauto. rewrite in_map_iff; eauto. }
+      { admit "use determinacy of find_fptr_owner_determ". }
+    }
   Qed.
 
 
 
-  Lemma find_fptr_owner_bsim_without_sim_skenv_def_bsim
+  Lemma find_fptr_owner_bsim
         sm0 ge_src ge_tgt
         (SIMGE: sim_ge sm0 ge_src ge_tgt)
         fptr_src fptr_tgt
@@ -193,30 +428,47 @@ Section SIMGE.
         /\ <<SIMSKENV: ModSemPair.sim_skenv msp sm0>>
   .
   Proof.
-    inv SIMGE.
-    rewrite Forall_forall in *.
-    dup SAFESRC.
-    inv SAFESRC.
-    rewrite in_map_iff in MODSEM. des. rename x into msp.
-    specialize (SIMMSS msp). exploit SIMMSS; eauto. clear SIMMSS. intro SIMMS.
-    specialize (SIMSKENV msp). exploit SIMSKENV; eauto. clear SIMSKENV. intro SIMSKENV.
+  (*   inv SIMGE. *)
+  (*   rewrite Forall_forall in *. *)
+  (*   clear SAFESRC. *)
+  (*   inv FINDTGT. *)
+  (*   rewrite in_map_iff in MODSEM. des. rename x into msp. *)
+  (*   specialize (SIMMSS msp). exploit SIMMSS; eauto. clear SIMMSS. intro SIMMS. *)
+  (*   specialize (SIMSKENV msp). exploit SIMSKENV; eauto. clear SIMSKENV. intro SIMSKENV. *)
+  (*   clarify. *)
+  (*   esplits; eauto. *)
 
-    assert(exists blk_tgt, fptr_tgt = Vptr blk_tgt Ptrofs.zero true).
-    { inv FINDTGT. esplits; eauto. } des. clarify.
-    exploit SimSymb.sim_skenv_def_fsim; eauto. intro SIMDEF; des.
-    inv SIMDEF. exploit DEFFSIM; eauto. i; des. clear_tac. inv SIM. inv SIM0.
 
-    assert(FINDSRC: Ge.find_fptr_owner (map ModSemPair.tgt msps)
-                                       (Vptr blk_tgt Ptrofs.zero true) msp.(ModSemPair.tgt)).
-    { econs; eauto. rewrite in_map_iff. esplits; eauto. }
-    esplits; eauto.
-    assert(exists tp tsk, tp.(Sem.semantics).(globalenv) = (map ModSemPair.tgt msps) /\ link_sk tp = Some tsk).
-    { admit "". }
-    des.
-    eapply find_fptr_owner_determ with (p:= tp); eauto.
-    { ss. des_ifs. rewrite H. eauto. }
-    { ss. des_ifs. rewrite H. eauto. }
-  Qed.
+  (*   inv SIMGE. *)
+  (*   rewrite Forall_forall in *. *)
+  (*   dup SAFESRC. *)
+  (*   inv SAFESRC. *)
+  (*   rewrite in_map_iff in MODSEM. des. rename x into msp. *)
+  (*   specialize (SIMMSS msp). exploit SIMMSS; eauto. clear SIMMSS. intro SIMMS. *)
+  (*   specialize (SIMSKENV msp). exploit SIMSKENV; eauto. clear SIMSKENV. intro SIMSKENV. *)
+
+  (*   inv FINDTGT. rewrite in_map_iff in *. des. rename msp into _msp. rename x into msp. clarify. *)
+  (*   exploit SimSymb.sim_skenv_func_bsim; eauto. intro SIMFUNC; des. *)
+  (*   inv SIMFUNC. exploit FUNCBSIM; eauto. i; des. clear_tac. inv SIM. *)
+  (*   ttttttttttt *)
+
+  (*   assert(exists blk_tgt, fptr_tgt = Vptr blk_tgt Ptrofs.zero true). *)
+  (*   { inv FINDTGT. esplits; eauto. } des. clarify. *)
+  (*   exploit SimSymb.sim_skenv_def_fsim; eauto. intro SIMDEF; des. *)
+  (*   inv SIMDEF. exploit DEFFSIM; eauto. i; des. clear_tac. inv SIM. inv SIM0. *)
+
+  (*   assert(FINDSRC: Ge.find_fptr_owner (map ModSemPair.tgt msps) *)
+  (*                                      (Vptr blk_tgt Ptrofs.zero true) msp.(ModSemPair.tgt)). *)
+  (*   { econs; eauto. rewrite in_map_iff. esplits; eauto. } *)
+  (*   esplits; eauto. *)
+  (*   assert(exists tp tsk, tp.(Sem.semantics).(globalenv) = (map ModSemPair.tgt msps) /\ link_sk tp = Some tsk). *)
+  (*   { admit "". } *)
+  (*   des. *)
+  (*   eapply find_fptr_owner_determ with (p:= tp); eauto. *)
+  (*   { ss. des_ifs. rewrite H. eauto. } *)
+  (*   { ss. des_ifs. rewrite H. eauto. } *)
+  (* Qed. *)
+  Abort.
 
 
 
@@ -233,7 +485,9 @@ Section SIMGE.
   Proof.
     inv INSRC. inv INTGT.
     inv SIMGE.
+    { ss. }
     rewrite Forall_forall in *.
+    { 
     rewrite in_map_iff in *. des.
   Abort.
 
@@ -247,9 +501,9 @@ Section SIMGE.
   .
   Proof.
     inv SIMGE.
-    econs; eauto.
+    { econs; eauto. }
+    econs 2; try reflexivity; eauto.
     rewrite Forall_forall in *. ii.
-    u.
     eapply SimSymb.mle_preserves_sim_skenv; eauto.
     eapply SIMSKENV; eauto.
   Qed.
@@ -262,7 +516,8 @@ Section SIMGE.
   .
   Proof.
     inv SIMGE.
-    econs; eauto.
+    { econs; eauto. }
+    econs 2; try reflexivity; eauto.
     rewrite Forall_forall in *. ii.
     u.
     eapply SimSymb.mlift_preserves_sim_skenv; eauto.
@@ -296,7 +551,7 @@ Section ADQMATCH.
   Hypothesis LINKTGT: (link_sk p_tgt) = Some sk_link_tgt.
   Let sem_src := Sem.semantics p_src.
   Let sem_tgt := Sem.semantics p_tgt.
-  Compute sem_src.(state).
+  Compute sem_src.(Smallstep.state).
 
   Print Frame.t.
   (* Record t : Type := mk { ms : ModSem.t;  lst : ModSem.state ms;  rs_init : regset } *)
@@ -306,7 +561,7 @@ Section ADQMATCH.
   (* Simulation can go continuation when SimMem.t bigger than argument is given, (after unlifting it) *)
   (* with after_external fed with regsets sent. *)
   Inductive lxsim_stack: regset -> regset -> SimMem.t ->
-                         sem_src.(state) -> sem_tgt.(state) -> Prop :=
+                         sem_src.(Smallstep.state) -> sem_tgt.(Smallstep.state) -> Prop :=
   | lxsim_stack_nil
       rs_init_src rs_init_tgt sm0
     :
@@ -358,7 +613,7 @@ Section ADQMATCH.
 
   .
 
-  Inductive lxsim_lift: idx -> sem_src.(state) -> sem_tgt.(state) -> SimMem.t -> Prop :=
+  Inductive lxsim_lift: idx -> sem_src.(Smallstep.state) -> sem_tgt.(Smallstep.state) -> SimMem.t -> Prop :=
   | lxsim_lift_intro
       sm0
       (GE: sim_ge sm0 sem_src.(globalenv) sem_tgt.(globalenv))
@@ -402,16 +657,211 @@ Section ADQINIT.
   Let p_src := pp.(ProgPair.src).
   Let p_tgt := pp.(ProgPair.tgt).
   Let lxsim_lift := (@lxsim_lift _ _ p_src p_tgt).
+  Hint Unfold lxsim_lift.
   Let sem_src := Sem.semantics p_src.
   Let sem_tgt := Sem.semantics p_tgt.
   Print Sem.initial_state.
 
-  Theorem init_lxsim_lift
+  Theorem init_sim_ge
+    :
+      exists sm_init, <<SIMGE: sim_ge sm_init sem_src.(globalenv) sem_tgt.(globalenv)>>
+               /\ <<MWF: SimMem.wf sm_init>>
+  .
+  Proof.
+    ss. subst_locals.
+    destruct (link_sk (ProgPair.src pp)) eqn:LINKSRC; cycle 1.
+    { esplits; eauto.
+      - econs 1; eauto.
+      - admit "there is SimMem.bot, which is wf".
+    }
+    rename t into sk_link_src.
+    (* { u. *)
+    (*   ginduction pp; ii; ss. *)
+    (*   destruct a; ss. *)
+    (*   unfold ProgPair.src in *. *)
+    (*   unfold link_sk in *. ss. *)
+    (*   eapply link_list_cons_inv in LINKSRC. des. *)
+    (*   rename sk_link_src into sk_link_link_src. *)
+    (*   rename restl into sk_link_src. *)
+    (*   inv SIMPROG. *)
+    (*   exploit IHt; eauto. intro IH; des. inv IH. *)
+    (*   inv H1. ss. *)
+    (*   exploit SimSymb.sim_sk_link. *)
+    (*   { apply SIMSK. } *)
+    (*   { apply IH0. } *)
+    (*   { eauto. } *)
+    (*   i; des. *)
+    (*   esplits; eauto. *)
+    (*   - eapply link_list_cons; eauto. *)
+    (*   - econs; eauto. *)
+    (*     rewrite Forall_forall in *. *)
+    (*     ii. *)
+    (*     all ltac:(fun H => apply link_list_linkorder in H). des. *)
+    (*     rewrite Forall_forall in *. *)
+    (*     eapply SimSymb.le_trans; eauto. *)
+    (*     + eapply TL; eauto. *)
+    (*       destruct x; ss. *)
+    (*       apply in_map_iff. esplits; ss; eauto. *)
+    (*       apply in_map_iff. esplits; ss; eauto. ss. *)
+    (*     + eapply IH; eauto. *)
+    (*       destruct x; ss. *)
+    (*       apply in_map_iff. esplits; ss; eauto. *)
+    (*       apply in_map_iff. esplits; ss; eauto. ss. *)
+    (* } *)
+
+
+  (*   exploit sim_link_sk; eauto. i; des. des_ifs. *)
+  (*   unfold link_sk in *. *)
+  (*   esplits; eauto. *)
+
+  (*   ginduction pp; ii; ss. *)
+  (*   destruct a; ss. *)
+  (*   inv LE. inv SIMPROG. ss. *)
+  (*   apply link_list_cons_inv in LINKSRC. apply link_list_cons_inv in Heq. *)
+  (*   des. *)
+  (*   exploit SimSymb.sim_sk_link. *)
+  (*   { *)
+  (*   exploit IHt; eauto. *)
+  (*   esplits; eauto. *)
+  (*   econs; cycle 2. *)
+  (*   { u. *)
+  (*     instantiate (1:= (ModSemPair.mk _ _ _ _) :: _). ss. *)
+  (*     f_equal. *)
+  (*     unfold ModSemPair.src. ss. u. *)
+  (*     Check (@ModSemPair.mk SM SS _ _ _ _ _). *)
+  (* Qed. *)
+  Admitted.
+
+  Theorem init_sim_ge_strong
+          sk_link_src sk_link_tgt
+          (SKSRC: link_sk p_src = Some sk_link_src)
+          (SKTGT: link_sk p_tgt = Some sk_link_tgt)
+          skenv_link_src skenv_link_tgt
+          (SKENVSRC: Sk.load_skenv sk_link_src = skenv_link_src)
+          (SKENVTGT: Sk.load_skenv sk_link_tgt = skenv_link_tgt)
+          m_src
+          (LOADSRC: Sk.load_mem sk_link_src = Some m_src)
+    :
+      exists sm_init ss_link, <<SIMGE: sim_ge sm_init sem_src.(globalenv) sem_tgt.(globalenv)>>
+               /\ <<MWF: SimMem.wf sm_init>>
+               /\ <<LOADTGT: Sk.load_mem sk_link_tgt = Some sm_init.(SimMem.tgt_mem)>>
+               /\ <<MSRC: sm_init.(SimMem.src_mem) = m_src>>
+               /\ <<SIMSKENV: SimSymb.sim_skenv sm_init ss_link skenv_link_src skenv_link_tgt>>
+  .
+  Admitted.
+
+  Theorem init_lxsim_lift_progress
           st_init_src
-          (INITSRC: sem_src.(initial_state) st_init_src)
+          (INITSRC: sem_src.(Smallstep.initial_state) st_init_src)
+    :
+      exists st_init_tgt,
+        <<INITTGT: sem_tgt.(Smallstep.initial_state) st_init_tgt>>
+  .
+  Proof.
+    inv INITSRC; ss.
+    rename sk_link into sk_link_src.
+    rename st_init into st_init_src.
+    rename ms into ms_src. rename m into m_src.
+    rename INIT into INITSRC. rename INITSK into INITSKSRC. rename INITMEM into INITMEMSRC.
+    (* inv MSFIND. *)
+    (* rename blk into blk_src. rename if_sig into if_sig_src. rename FPTR into FPTRSRC. *)
+    (* rename MODSEM into MODSEMSRC. rename INTERNAL into INTERNALSRC. *)
+
+    exploit sim_link_sk; eauto. i; des. fold p_tgt in LOADTGT.
+    exploit init_sim_ge_strong; eauto. i; des. clarify.
+    ss. des_ifs.
+
+    assert(SIMFPTR: SimMem.sim_val sm_init (Genv.symbol_address (Genv.globalenv sk_link_src)
+                                                                (prog_main sk_link_src) Ptrofs.zero)
+                                   (Genv.symbol_address (Genv.globalenv sk_link_tgt)
+                                                        (prog_main sk_link_tgt) Ptrofs.zero)).
+    { admit "strengthen sim_skenv specs". }
+
+    exploit find_fptr_owner_fsim; eauto. i; des. clarify.
+    inv SIMMS.
+    inv MSFIND. inv FINDTGT.
+    assert(SIMRS: SimMem.sim_regset sm_init
+        (init_regs (Genv.symbol_address (Sk.load_skenv sk_link_src) (prog_main sk_link_src) Ptrofs.zero))
+        (init_regs (Genv.symbol_address (Sk.load_skenv sk_link_tgt) (prog_main sk_link_tgt) Ptrofs.zero))).
+    { u. ii. ss.
+      unfold Pregmap.set.
+      des_ifs.
+      - admit "strengthen sim_val".
+      - admit "strengthen sim_val".
+      - admit "strengthen sim_val".
+    }
+    exploit SIM; eauto. i; des.
+    bar.
+    exploit INITPROGRESS; eauto. i; des.
+    esplits; eauto. econs; eauto. econs; eauto.
+  Qed.
+
+  Theorem init_lxsim_lift_backward
+          st_init_tgt
+          (INITTGT: sem_tgt.(Smallstep.initial_state) st_init_tgt)
+          (SAFESRC: __guard__ (exists _st_init_src, sem_src.(Smallstep.initial_state) _st_init_src))
+    :
+      exists idx st_init_src sm_init,
+        <<INITTGT: sem_src.(Smallstep.initial_state) st_init_src>>
+        /\ <<SIM: lxsim_lift idx st_init_src st_init_tgt sm_init>>
+  .
+  Proof.
+    (* inv SAFESRC; ss. *)
+    (* rename sk_link into sk_link_src. *)
+    (* rename st_init into st_init_src. *)
+    (* rename ms into ms_src. rename m into m_src. *)
+    (* rename INIT into INITSRC. rename INITSK into INITSKSRC. rename INITMEM into INITMEMSRC. *)
+    assert(exists sk_link_src m_src, <<INITSKSRC: link_sk p_src = Some sk_link_src>>
+                                                  /\ <<LOADSRC: Sk.load_mem sk_link_src = Some m_src>>).
+    { unguard. des. inv SAFESRC. esplits; eauto. } des.
+
+    exploit sim_link_sk; eauto. i; des. fold p_tgt in LOADTGT.
+    exploit init_sim_ge_strong; eauto. i; des. clarify.
+    ss. des_ifs.
+
+    assert(SIMFPTR: SimMem.sim_val sm_init (Genv.symbol_address (Genv.globalenv sk_link_src)
+                                                                (prog_main sk_link_src) Ptrofs.zero)
+                                   (Genv.symbol_address (Genv.globalenv sk_link_tgt)
+                                                        (prog_main sk_link_tgt) Ptrofs.zero)).
+    { admit "strengthen sim_skenv specs". }
+
+    inv INITTGT. clarify.
+    exploit find_fptr_owner_bsim_deprecated; eauto.
+    { unguard. des. inv SAFESRC. clarify. esplits; eauto. } i; des. clarify.
+    inv SIMMS.
+    inv MSFIND. inv FINDSRC.
+    assert(SIMRS: SimMem.sim_regset sm_init
+        (init_regs (Genv.symbol_address (Sk.load_skenv sk_link_src) (prog_main sk_link_src) Ptrofs.zero))
+        (init_regs (Genv.symbol_address (Sk.load_skenv sk_link_tgt) (prog_main sk_link_tgt) Ptrofs.zero))).
+    { u. ii. ss.
+      unfold Pregmap.set.
+      des_ifs.
+      - admit "strengthen sim_val".
+      - admit "strengthen sim_val".
+      - admit "strengthen sim_val".
+    }
+    bar.
+    exploit SIM; eauto. i; des. clear INITPROGRESS.
+    exploit INITSIM; eauto. i; des. clear INITSIM.
+
+    destruct msp; ss.
+    assert(idx = Ord.idx). { admit "easy". } clarify.
+    assert(ord = Ord.ord). { admit "easy". } clarify.
+
+    esplits; eauto.
+    - econs; eauto. econs; eauto.
+    - econs; eauto.
+      + ss. des_ifs.
+      + econs; eauto.
+      + reflexivity.
+  Qed.
+
+  Theorem init_lxsim_lift_forward
+          st_init_src
+          (INITSRC: sem_src.(Smallstep.initial_state) st_init_src)
     :
       exists idx st_init_tgt sm_init,
-        <<INITTGT: sem_tgt.(initial_state) st_init_tgt>>
+        <<INITTGT: sem_tgt.(Dinitial_state) st_init_tgt>>
         /\ <<SIM: lxsim_lift idx st_init_src st_init_tgt sm_init>>
   .
   Proof.
@@ -424,31 +874,47 @@ Section ADQINIT.
     (* rename blk into blk_src. rename if_sig into if_sig_src. rename FPTR into FPTRSRC. *)
     (* rename MODSEM into MODSEMSRC. rename INTERNAL into INTERNALSRC. *)
 
-    exploit sim_link_sk; eauto. i; des.
-    exploit SimSymb.sim_sk_load_sim_skenv; eauto. i; des.
+    exploit sim_link_sk; eauto. i; des. fold p_tgt in LOADTGT.
+    exploit init_sim_ge_strong; eauto. i; des. clarify.
+    ss. des_ifs.
 
-    esplits; eauto.
-    - econs; eauto.
-      + econs; eauto.
-    -
+    assert(SIMFPTR: SimMem.sim_val sm_init (Genv.symbol_address (Genv.globalenv sk_link_src)
+                                                                (prog_main sk_link_src) Ptrofs.zero)
+                                   (Genv.symbol_address (Genv.globalenv sk_link_tgt)
+                                                        (prog_main sk_link_tgt) Ptrofs.zero)).
+    { admit "strengthen sim_skenv specs". }
 
-    inv INITTGT; ss.
-    rename sk_link into sk_link_tgt.
-    rename st_init into st_init_tgt.
-    rename ms into ms_tgt. rename m into m_tgt.
-    inv INITSRC; ss.
-
-    assert(MEM: exists sm: SimMem.t, True).
-    { admit "". }
-    des.
-    assert(GE: sim_ge sm (load_genv p_src (Sk.load_skenv sk_link)) (load_genv p_src (Sk.load_skenv sk_link))).
-    {
-      u.
-      econs; eauto.
+    exploit find_fptr_owner_fsim; eauto. i; des. clarify.
+    inv SIMMS.
+    inv MSFIND. inv FINDTGT.
+    assert(SIMRS: SimMem.sim_regset sm_init
+        (init_regs (Genv.symbol_address (Sk.load_skenv sk_link_src) (prog_main sk_link_src) Ptrofs.zero))
+        (init_regs (Genv.symbol_address (Sk.load_skenv sk_link_tgt) (prog_main sk_link_tgt) Ptrofs.zero))).
+    { u. ii. ss.
+      unfold Pregmap.set.
+      des_ifs.
+      - admit "strengthen sim_val".
+      - admit "strengthen sim_val".
+      - admit "strengthen sim_val".
     }
-    exploit find_fptr_owner_bsim; eauto.
+    exploit SIM; eauto. i; des.
+    bar.
+    exploit INITPROGRESS; eauto. i; des.
+    bar.
+    exploit find_fptr_owner_fsim; eauto. { econs; eauto. } i; des.
+
+    remember (ModSemPair.src msp) as srcm. revert Heqsrcm. clarify. i. clears msp.
+
+    inv SIMMS. inv FINDTGT.
+    exploit SIM; eauto. i; des.
+    exploit INITSIM; eauto. i; des.
+
     esplits; eauto.
-    econs; eauto.
+    - econs; ss; cycle 1.
+      { ii. eapply initial_state_determ; ss; eauto. }
+      econs; eauto.
+      u.
+    -
   Qed.
 
   Theorem init_progress
