compose/SimSymbDrop.v
@@ -448,9 +448,32 @@ Qed.
 Next Obligation.
   inv SIMSKENV.
   econs; eauto.
+  ii. ss. inv SIMFPTR; ss.
+  des_ifs_safe; ss. unfold Genv.find_funct_ptr in *. des_ifs_safe.
+  exploit SIMDEF; eauto. i; des.
+  inv SIM.
+  rewrite DEFTGT.
+  esplits; eauto.
+  des_ifs.
 Qed.
 Next Obligation.
   inv SIMSKENV.
   econs; eauto.
+  -
+    ii. ss. inv SIMFPTR; ss; cycle 1.
+    { des. ss. }
+    clear SAFESRC.
+    des_ifs_safe; ss. unfold Genv.find_funct_ptr in *. des_ifs_safe.
+    exploit SIMDEFINV; eauto. i; des.
+    inv SIM.
+    rewrite DEFSRC.
+    esplits; eauto.
+    des_ifs.
+    exfalso.
+    apply n.
+    rewrite Ptrofs.add_zero_l in *. rewrite DELTA in *. rewrite Ptrofs.add_zero in *. clarify.
+  -
+    ii. des. ss. inv SIMFPTR; ss. des_ifs_safe. unfold Genv.find_funct_ptr in *. des_ifs_safe.
+    exploit SIMDEF; eauto. i; des. des_ifs_safe. inv SIM. esplits; eauto.
 Qed.
 
